Fix DVE for mutual

DVE.v
@@ -90,18 +90,14 @@ Proof.
   revert_except s.
   sind s; destruct s; simpl; intros; invt true_live_sound; simpl in * |- *.
   - case_eq (exp_eval V e); intros. cases.
-    + pfold. econstructor; try eapply plus2O.
-      econstructor; eauto. reflexivity.
-      econstructor; eauto. instantiate (1:=v).
-      erewrite exp_eval_live; eauto. eapply agree_on_sym; eauto. reflexivity.
-      left. eapply (IH s); eauto. eapply agree_on_update_same. reflexivity.
-      eapply agree_on_incl; eauto.
+    + pone_step.
+      instantiate (1:=v). erewrite exp_eval_live; eauto. eapply agree_on_sym; eauto.
+      left. eapply (IH s); eauto. eapply agree_on_update_same; eauto with cset.
     + eapply sim'_expansion_closed;
       [ | eapply S_star2 with (y:=EvtTau);
           [ econstructor; eauto | eapply star2_refl ]
         | eapply star2_refl].
-      eapply (IH s); eauto. eapply agree_on_update_dead; eauto.
-      eapply agree_on_incl; eauto. rewrite <- H9. cset_tac; intuition.
+      eapply (IH s); eauto. eapply agree_on_update_dead; eauto with cset.
     + pfold. econstructor 3; [| eapply star2_refl|]; eauto. stuck.
   - repeat cases.
     + edestruct (exp2bool_val2bool V); eauto; dcr.
@@ -121,16 +117,9 @@ Proof.
       exploit exp_eval_live_agree; eauto.
       eapply H8. case_eq (exp2bool e); intros; try destruct b; congruence.
       destruct o. case_eq (val2bool v); intros.
-      pfold; econstructor; try eapply plus2O.
-      econstructor; eauto. reflexivity.
-      econstructor; eauto. reflexivity.
-      left; eapply (IH s1); eauto using agree_on_incl.
-      pfold; econstructor; try eapply plus2O.
-      econstructor 3; eauto. reflexivity.
-      econstructor 3; eauto. reflexivity.
-      left; eapply (IH s2); eauto using agree_on_incl.
-      pfold. econstructor 3; try eapply star2_refl; eauto.
-      stuck.
+      pone_step. left. eapply IH; eauto with cset.
+      pone_step. left; eapply (IH s2); eauto with cset.
+      pno_step.
   - destruct (get_dec L (counted l)) as [[[bE bZ bs]]|].
     + remember (omap (exp_eval V) Y). symmetry in Heqo.
       rewrite (get_nth (∅, nil) H4); simpl.
@@ -147,9 +136,7 @@ Proof.
       * pfold; econstructor 3; try eapply star2_refl; eauto; stuck2.
     + pfold; econstructor 3; try eapply star2_refl; eauto; stuck2.
       hnf in H1. inRel_invs. eauto.
-  - pfold. econstructor 4; try eapply star2_refl.
-    simpl. erewrite <- exp_eval_live_agree; eauto. eapply agree_on_sym; eauto.
-    stuck2. stuck2.
+  - pno_step; simpl. erewrite <- exp_eval_live_agree; eauto; symmetry; eauto.
   - pfold.
     remember (omap (exp_eval V) Y). symmetry in Heqo.
     exploit omap_exp_eval_live_agree; eauto.
@@ -167,11 +154,7 @@ Proof.
         eapply agree_on_incl; eauto.
     + eapply sim'Err; try eapply star2_refl; simpl; eauto.
       stuck2.
-  - pfold. econstructor; try eapply plus2O.
-    econstructor; eauto. reflexivity.
-    econstructor; eauto. reflexivity.
-    simpl. left. eapply IH; eauto.
-    + simpl in *; eapply agree_on_incl; eauto.
+  - pone_step. left. eapply IH; eauto with cset.
     + eapply simL_mon; eauto. eapply simL_extension'; eauto with len.
       * intros. inv_get; simpl. split. hnf; intros; simpl.
         unfold ParamRel, ArgRel. intuition.
@@ -222,10 +205,8 @@ Proof.
   revert_except s.
   sind s; destruct s; simpl; intros; invt true_live_sound; simpl in * |- *.
   - case_eq (exp_eval V e); intros. cases.
-    + pfold. econstructor; try eapply plus2O.
-      econstructor; eauto. reflexivity.
-      econstructor; eauto. instantiate (1:=v).
-      erewrite exp_eval_live; eauto. eapply agree_on_sym; eauto. reflexivity.
+    + pone_step. instantiate (1:=v).
+      erewrite exp_eval_live; eauto. eapply agree_on_sym; eauto.
       left. eapply (IH s); eauto. eapply agree_on_update_same. reflexivity.
       eapply agree_on_incl; eauto.
     + eapply sim'_expansion_closed;
@@ -345,11 +326,9 @@ Fixpoint compile_live (s:stmt) (a:ann (set var)) (G:set var) : ann (set var) :=
     | stmtExtern x f Y s, ann1 lv an as a =>
       ann1 (G ∪ lv) (compile_live s an {x})
     | stmtFun F t, annF lv ans ant =>
-      let ans' := zip (fun Zs a => compile_live (snd Zs) a ∅) F ans in
-      ann2 (G ∪ lv) (setTopAnn (ans')
-                           (getAnn ans' ∪
-                                   of_list (List.filter (fun x => B[x ∈ getAnn ans]) Z)))
-                           (compile_live t ant ∅)
+      let ans' := zip (fun Zs a => let a' := compile_live (snd Zs) a ∅ in
+                               setTopAnn a' (getAnn a' ∪ of_list (List.filter (fun x => B[x ∈ getAnn a]) (fst Zs)))) F ans in
+      annF (G ∪ lv) ans' (compile_live t ant ∅)
     | _, a => a
   end.
 
@@ -358,12 +337,12 @@ Lemma compile_live_incl G i LV s lv
   : true_live_sound i LV s lv
     -> getAnn (compile_live s lv G) ⊆ G ∪ getAnn lv.
 Proof.
-  intros. general induction H; simpl; eauto; try (now (cset_tac; intuition)).
+  intros. general induction H; simpl; eauto.
   - cases; simpl; try reflexivity.
     rewrite IHtrue_live_sound. rewrite <- H1. cset_tac; intuition.
   - repeat cases; simpl; try reflexivity.
-    + etransitivity; eauto. rewrite <- H2. reflexivity. congruence.
-    + etransitivity; eauto.  rewrite <- H3. reflexivity. congruence.
+    + etransitivity; eauto. rewrite <- H2. eauto. congruence.
+    + etransitivity; eauto.  rewrite <- H3; eauto.
 Qed.
 
 Lemma compile_live_incl_empty i LV s lv
@@ -379,27 +358,11 @@ Lemma incl_compile_live G i LV s lv
   : true_live_sound i LV s lv
     -> G ⊆ getAnn (compile_live s lv G).
 Proof.
-  intros. general induction H; simpl; eauto; try (now (cset_tac; intuition)).
+  intros. general induction H; simpl; eauto.
   - cases; simpl; try reflexivity. cset_tac; intuition.
     rewrite <- IHtrue_live_sound. cset_tac; intuition.
   - repeat cases; simpl; try reflexivity; eauto.
 Qed.
-
-
-(*
-Lemma compile_live_incl' i LV s lv
-  : true_live_sound i LV s lv
-    -> getAnn lv ⊆ getAnn (compile_live s lv).
-Proof.
-  intros. general induction H; simpl; eauto; try reflexivity.
-  - cases; simpl; try reflexivity.
-    rewrite <- IHtrue_live_sound.
-    rewrite H2; eauto.
-  - repeat cases; simpl; try reflexivity.
-    + etransitivity; eauto.
-    + etransitivity; eauto.
-Qed.
- *)
 
 Definition compile_LV (LV:list (set var *params)) :=
   List.map (fun lvZ => let Z' := List.filter (fun x => B[x ∈ fst lvZ]) (snd lvZ) in
@@ -411,7 +374,7 @@ Lemma dve_live i LV s lv G
 Proof.
   intros. general induction H; simpl; eauto using live_sound, compile_live_incl.
   - cases; eauto. econstructor; eauto.
-    + eapply live_exp_sound_incl; eauto. cset_tac; intuition.
+    + eapply live_exp_sound_incl; eauto. eauto.
     + rewrite compile_live_incl; eauto.
       rewrite <- H1. cset_tac; intuition.
     + eapply incl_compile_live; eauto.
@@ -444,27 +407,28 @@ Proof.
     + intros; eapply live_exp_sound_incl; eauto using incl_right.
     + rewrite compile_live_incl; eauto. rewrite <- H1. cset_tac; intuition.
     + eapply incl_compile_live; eauto.
-  - econstructor; simpl in *.
-    eapply live_sound_monotone. eapply live_sound_monotone2.
-    eapply IHtrue_live_sound1. cset_tac; intuition.
-    econstructor; simpl.
-    simpl. rewrite getAnn_setTopAnn, compile_live_incl.
-    split; eauto. rewrite filter_incl. cset_tac; intuition.
-    eauto. eapply PIR2_refl. hnf; intuition.
-    eapply live_sound_monotone. eapply IHtrue_live_sound2.
-    econstructor; simpl.
-    rewrite getAnn_setTopAnn, compile_live_incl.
-    split; eauto. rewrite filter_incl. cset_tac; intuition. eauto.
-    eapply PIR2_refl. hnf; intuition.
-    rewrite getAnn_setTopAnn. cset_tac; intuition.
-    rewrite getAnn_setTopAnn.
-    cases; simpl in * |- *; eauto.
-    rewrite compile_live_incl; eauto.
-    rewrite union_comm. rewrite union_minus_remove.
-    rewrite <- H1.
-    rewrite minus_inter_empty. instantiate (1:=of_list Z).
-    cset_tac; intuition.
-    cset_tac; intuition. eapply filter_incl2; eauto.
-    eapply filter_in; eauto. intuition. hnf. cases; eauto.
-    rewrite compile_live_incl; eauto. cset_tac; intuition.
+  - econstructor; simpl in *; eauto with len.
+    + eapply live_sound_monotone.
+      eapply IHtrue_live_sound.
+      unfold compile_LV. rewrite map_app. eapply PIR2_app; eauto.
+      eapply PIR2_get; eauto 30 with len.
+      intros; inv_get. simpl. rewrite getAnn_setTopAnn.
+      rewrite compile_live_incl_empty; eauto. rewrite of_list_filter.
+      split; cset_tac.
+    + intros; inv_get.
+      eapply live_sound_monotone.
+      eapply live_sound_monotone2; eauto. eapply H2; eauto.
+      unfold compile_LV. rewrite map_app. eapply PIR2_app; eauto.
+      eapply PIR2_get; eauto 30 with len.
+      intros; inv_get. simpl. rewrite getAnn_setTopAnn.
+      rewrite compile_live_incl_empty; eauto. rewrite of_list_filter.
+      split; cset_tac.
+    + intros; inv_get.
+      repeat rewrite getAnn_setTopAnn; simpl.
+      split; eauto. cases; eauto.
+      exploit H3; eauto.
+      rewrite compile_live_incl_empty; eauto. rewrite <- H5.
+      rewrite of_list_filter.
+      clear_all; cset_tac.
+    + rewrite compile_live_incl; eauto with cset.
 Qed.
