ValueOpts.v
@@ -3,7 +3,7 @@ Require Import CSet Le.
 Require Import Plus Util AllInRel Map.
 Require Import CSet Val Var Env EnvTy Equiv.Sim IL Fresh Annotation MoreExp Coherence RenamedApart.
 
-Require Import SetOperations Liveness Filter Eqn.
+Require Import SetOperations Liveness Eqn.
 
 Set Implicit Arguments.
 Unset Printing Records.
